WIP: improve eval

dataplane/Examples/Batch_op_Correctness.thy
@@ -29,11 +29,13 @@ abbreviation "t1 \<equiv> MyPair (Suc 0) (0 :: nat)"
 abbreviation "t2 \<equiv> MyPair (0 :: nat) (Suc 0)"
 abbreviation "t3 \<equiv> MyPair (Suc 0) (Suc 0)"
 
-abbreviation "inps1 \<equiv> llist_of [Data 0 0, Data (0 :: nat) (42 :: nat), Data 1 43]"
+abbreviation "inps1 \<equiv> llist_of [Data 1 4, Data (0 :: nat) (10 :: nat), Data 0 0, Data 2 11]"
 
-abbreviation "inps2 \<equiv> llist_of [Mint t1, Mint t2, Mint t3, Data t3 42, Drop t3, Data t2 7, Data t1 (-2 :: int), Data t2 (-1), Data t1 (- 3), Drop t1, Drop t2]"
+abbreviation "inps2 \<equiv> llist_of [Mint t1, Mint t2, Mint t3, Data t3 10, Drop t3, Data t2 7, Data t1 (-2 :: int), Data t2 (-1), Data t1 (- 3), Drop t1, Drop t2]"
 
 value \<open>list_of (lconcat (batch_fun_spec (\<lambda> b. [Max (set b)]) inps1 [] []))\<close>
+value \<open>list_of (lconcat (batch_fun_spec (\<lambda> b. [Max (set b)]) inps1 [] []))\<close>
+
 value \<open>list_of (lconcat (batch_fun_spec (\<lambda> b. [Max (set b)]) inps2 [] []))\<close>
 
 abbreviation init_input_state where
@@ -80,10 +82,78 @@ lemma one_plus[code]:
   "(1 :: 1) + x = 1"
   by auto
 
-definition "my_test = approx_in 23 [VOut (1, 1) (Inr 42, 0), VOut (1, 1) (Inr 43, 1)] dt"
+find_theorems eval'
+
+find_theorems cset_of_llist cUnion
+
+partial_function (llist) lrmdups_aux where
+  "lrmdups_aux f S lxs = (case lxs of LNil \<Rightarrow> LNil | LCons x lxs \<Rightarrow> (if f x \<in> S then lrmdups_aux f S lxs else LCons x (lrmdups_aux f (insert (f x) S) lxs)))"
+declare lrmdups_aux.simps[code]
+
+definition "lrmdups f = lrmdups_aux f {}"
+
+definition "compress_cfilter P xs = cfilter P xs"
+
+lemma compress_cfilter_code[code]: "compress_cfilter P (cset_of_llist xs) = cfilter P (cset_of_llist (lrmdups id xs))"
+  sorry
+
+friend_of_corec lappend where
+  "lappend xs lys = (case xs of LNil \<Rightarrow> (case lys of LNil \<Rightarrow> LNil | LCons x xs \<Rightarrow> LCons x xs)
+    | LCons x xs \<Rightarrow> LCons x (lappend xs lys))"
+  subgoal by (cases xs; cases lys; simp)
+  subgoal by transfer_prover
+  done
 
 
-value [GHC] "my_test"
+definition "my_eval = compress_cfilter ((\<noteq>) [])(eval 18 dt)"
+value [GHC] "my_eval" 
+ 
+definition "my_check = approx_in 20 [VOut (1, 1) (Inr 4, 1), VOut (1, 1) (Inr 10, 0)] dt"
+(* 
+definition "my_check = approx_in 24 [VOut (1, 1) (Inr 0, 0)] dt" *)
+(* 
+value [GHC] "my_check"
+ *)
+
+definition "rmdup_traces xs = xs"
+
+abbreviation "flat_choices ops \<equiv> cUnion (cimage choices ops)"
+
+find_consts "_ cset"
+
+context includes cset.lifting begin
+lift_definition ccard :: "'m cset \<Rightarrow> nat" is card .
+end
+
+term the_enat
+
+lemma ccard_code[code]:
+  "ccard (cset_of_llist xs) = the_enat (llength xs)"
+  sorry
+abbreviation "is_Visible x \<equiv> is_Write x \<or> is_Read x"
+
+abbreviation "optm ops \<equiv> let ops' = (cfilter (is_Visible o snd) ops) in if ccard ops' > 0 then ops' else ops"
+
+fun fast_eval' :: "nat \<Rightarrow> _ \<Rightarrow> _ \<Rightarrow> ('i, 'o, 'd :: {countable}) op \<Rightarrow> (('i, 'o, 'd) VIO list \<times> ('i, 'o, 'd) op) cset"  where
+  "fast_eval' 0 m i op = {|([], op)|}"
+| "fast_eval' n m 0 op = {||}"
+| "fast_eval' (Suc n) m i (Write op p x) = cimage (\<lambda>(t, op). (VOut p x # t, op)) (fast_eval' n m m op)"
+| "fast_eval' (Suc n) m i (Read p f) = cUnion (cimage (\<lambda>x. cimage (\<lambda>(t, op). (VInp p x # t, op)) (fast_eval' n m m (f x))) (cUNIV :: 'd cset))"
+| "fast_eval' n m (Suc i) (Silent op) = (cimage (\<lambda>(t, op). (t, op)) (fast_eval' n m i op))"
+| "fast_eval' n m (Suc i) (Choice ops) = (if ops = {||} then {|([], \<oslash>)|} else (let ops' = cUnion (cimage (fast_eval' n m i) ops) in optm ops'))"
+
+definition "fast_eval n m op = cimage fst (fast_eval' n m m op)"
+
+
+definition "my_fast_eval = compress_cfilter ((\<noteq>) []) (fast_eval 1 14 dt)"
+value [GHC] "my_fast_eval" 
+
+definition "fast_approx_in n m pfx op = 
+  (\<not> cis_empty (cfilter (\<lambda>xs. Sublist.prefix pfx xs) (cimage fst (fast_eval' n m m op))))"
+
+definition "my_fast_check = fast_approx_in 3 14 [VOut (1, 1) (Inr 4, 1), VOut (1, 1) (Inr 10, 0), VOut (1, 1) (Inr 11, 2)] dt"
+
+value [GHC] "my_fast_check" 
 
 
 (* export_code my_test in Haskell 
@@ -115,6 +185,7 @@ shows
 
   term outpos1
   term buf
+  oops
 
 
 end
